src/orders/minmax.v
@@ -4,82 +4,82 @@ Require Import
 
 (* This is ugly, maybe we should let TotalOrder live in Type to get rid of the Decision stuff *)
 Section contents.
-  Context `{Setoid A} `{Order A} `{prec_decide : ∀ x y: A, Decision (x ≤ y)}.
+  Context `{Setoid A} `{Order A} `{∀ x y: A, Decision (x ≤ y)}.
 
-  Definition sort (x y: A) : A * A := if prec_decide x y then (x, y) else (y, x).
+  Definition sort (x y: A) : A * A := if decide_rel (≤) x y then (x, y) else (y, x).
 
   Definition min (x y: A) := fst (sort x y).
   Definition max (x y: A) := snd (sort x y).
 
   Lemma min_lb_l x y `{!Reflexive (≤)} `{!TotalOrder (≤)} : min x y ≤ x.
-  Proof. unfold min, sort. case (prec_decide _); firstorder. Qed.
+  Proof. unfold min, sort. case (decide_rel _); firstorder. Qed.
 
   Lemma min_lb_r `{!Reflexive (≤)} x y : min x y ≤ y.
-  Proof. unfold min, sort. case (prec_decide _); firstorder. Qed.
+  Proof. unfold min, sort. case (decide_rel _); firstorder. Qed.
 
   Lemma min_l x y : x ≤ y → min x y = x.
-  Proof. unfold min, sort. case (prec_decide _); firstorder. Qed.
+  Proof. unfold min, sort. case (decide_rel _); firstorder. Qed.
 
   Lemma min_r `{!AntiSymmetric (≤)} x y : y ≤ x → min x y = y.
-  Proof. unfold min, sort. case (prec_decide _); firstorder. Qed.
+  Proof. unfold min, sort. case (decide_rel _); firstorder. Qed.
 
   Lemma min_diag x: min x x = x.
-  Proof. unfold min, sort. case (prec_decide _); reflexivity. Qed.
+  Proof. unfold min, sort. case (decide_rel _); reflexivity. Qed.
 
   Lemma max_ub_l `{!Reflexive (≤)} x y : x ≤ max x y.
-  Proof. unfold max, sort. case (prec_decide _); auto. Qed.
+  Proof. unfold max, sort. case (decide_rel _); auto. Qed.
 
   Lemma max_ub_r `{!Reflexive (≤)} `{!TotalOrder (≤)} x y : y ≤ max x y.
-  Proof. unfold max, sort. case (prec_decide _); firstorder. Qed.
+  Proof. unfold max, sort. case (decide_rel _); firstorder. Qed.
 
   Lemma max_l `{!AntiSymmetric (≤)} x y : y ≤ x → max x y = x.
-  Proof. unfold max, sort. case (prec_decide _); firstorder. Qed.
+  Proof. unfold max, sort. case (decide_rel _); firstorder. Qed.
 
   Lemma max_r x y : x ≤ y → max x y = y.
-  Proof. unfold max, sort. case (prec_decide _); firstorder. Qed.
+  Proof. unfold max, sort. case (decide_rel _); firstorder. Qed.
 
   Lemma max_diag x: max x x = x.
-  Proof. unfold max, sort. case (prec_decide _); reflexivity. Qed.
+  Proof. unfold max, sort. case (decide_rel _); reflexivity. Qed.
   
   Global Instance sort_proper `{!Proper ((=) ==> (=) ==> iff) (≤)} : Proper ((=) ==> (=) ==> (=)) sort.
-  Proof with assumption.
+  Proof.
     intros x y E x' y' E'.
     unfold sort.
-    do 2 case (prec_decide _); simpl.
+    do 2 case (decide_rel _); simpl.
         firstorder. 
-       intros F ?. destruct F. rewrite <-E, <-E'...
-      intros ? F. destruct F. rewrite E, E'...
+       intros F ?. destruct F. now rewrite <-E, <-E'.
+      intros ? F. destruct F. now rewrite E, E'.
     firstorder.
   Qed.
 
   Global Instance min_proper `{!Proper ((=) ==> (=) ==> iff) (≤)} : Proper ((=) ==> (=) ==> (=)) min.
-  Proof. unfold min. repeat intro. apply sm_proper. apply sort_proper; assumption. Qed.
+  Proof. unfold min. repeat intro. apply sm_proper. now apply sort_proper. Qed.
 
   Global Instance max_proper `{!Proper ((=) ==> (=) ==> iff) (≤)} : Proper ((=) ==> (=) ==> (=)) max.
-  Proof. unfold max. repeat intro. apply sm_proper. apply sort_proper; assumption. Qed.
+  Proof. unfold max. repeat intro. apply sm_proper. now apply sort_proper. Qed.
 
   Global Instance min_commutative `{!AntiSymmetric (≤)} `{!TotalOrder (≤)} : Commutative min.
-  Proof. intros x y. unfold min, sort. do 2 case (prec_decide _); firstorder. Qed.
+  Proof. intros x y. unfold min, sort. do 2 case (decide_rel _); firstorder. Qed.
 
   Global Instance max_commutative `{!AntiSymmetric (≤)} `{!TotalOrder (≤)} : Commutative max.
-  Proof. intros x y. unfold max, sort. do 2 case (prec_decide _); firstorder. Qed.
+  Proof. intros x y. unfold max, sort. do 2 case (decide_rel _); firstorder. Qed.
 
   Global Instance min_associative `{!AntiSymmetric (≤)} `{!Transitive (≤)} `{!TotalOrder (≤)} : Associative min.
-  Proof with auto; try reflexivity; try contradiction.
+  Proof.
      intros x y z. unfold min, sort.
-     case (prec_decide y z); simpl; intros E1; case (prec_decide x y); simpl; intros E2; 
-       case (prec_decide x z); simpl; intros E3; case (prec_decide y z); simpl; intros E4...
-     destruct E3. transitivity y...
-     destruct E4. transitivity x... apply orders.precedes_flip... 
+     case (decide_rel (≤) y z); simpl; intros E1; case (decide_rel (≤) x y); simpl; intros E2; 
+       case (decide_rel (≤) x z); simpl; intros E3; case (decide_rel (≤) y z); simpl; intros E4; try easy.
+     destruct E3. now transitivity y.
+     destruct E4. transitivity x. now apply orders.precedes_flip. easy.
   Qed.
 
   Global Instance max_associative `{!AntiSymmetric (≤)} `{!Transitive (≤)} `{!TotalOrder (≤)} : Associative max.
-  Proof with auto; try reflexivity; try contradiction.
+  Proof.
      intros x y z. unfold max, sort.
-     case (prec_decide y z); simpl; intros E1; case (prec_decide x y); simpl; intros E2; 
-       case (prec_decide x z); simpl; intros E3; case (prec_decide y z); simpl; intros E4...
-     destruct E3. transitivity y...
-     destruct E4. transitivity x... apply orders.precedes_flip... 
+     case (decide_rel (≤) y z); simpl; intros E1; case (decide_rel (≤) x y); simpl; intros E2; 
+       case (decide_rel (≤) x z); simpl; intros E3; case (decide_rel (≤) y z); simpl; intros E4; try easy.
+     destruct E3. now transitivity y.
+     destruct E4. transitivity x. now apply orders.precedes_flip. easy.
   Qed.
 End contents.
 
@@ -90,25 +90,25 @@ Instance: Params (@max) 3.
 Section order_preserving.
   Context `{PartialOrder A} `{PartialOrder B} {f : A → B} `{!OrderPreserving f}
     `{!TotalOrder (precedes (A:=A))} `{!TotalOrder (precedes (A:=B))}
-    `{prec_decideA : ∀ x y: A, Decision (x ≤ y)} `{prec_decideB : ∀ x y: B, Decision (x ≤ y)}. 
+    `{∀ x y: A, Decision (x ≤ y)} `{∀ x y: B, Decision (x ≤ y)}. 
 
-  Instance: Setoid A. apply poset_setoid. Qed.
-  Instance: Setoid B. apply poset_setoid. Qed.
+  Instance: Setoid A := poset_setoid.
+  Instance: Setoid B := poset_setoid.
 
   Lemma preserves_min x y : f (min x y) = min (f x) (f y).
-  Proof with auto.
+  Proof.
     symmetry. unfold min at 2. unfold sort.
-    case (prec_decideA _); simpl; intros E.
-     apply min_l. apply (order_preserving _)...
-    apply min_r. apply (order_preserving _). apply precedes_flip...
+    case (decide_rel _); simpl; intros E.
+     apply min_l. now apply (order_preserving _).
+    apply min_r. apply (order_preserving _). now apply precedes_flip.
   Qed.
 
   Lemma preserves_max x y : f (max x y) = max (f x) (f y).
-  Proof with auto.
+  Proof.
     symmetry. unfold max at 2. unfold sort.
-    case (prec_decideA _); simpl; intros E.
-     apply max_r. apply (order_preserving _)...
-    apply max_l. apply (order_preserving _). apply precedes_flip...
+    case (decide_rel _); simpl; intros E.
+     apply max_r. now apply (order_preserving _).
+    apply max_l. apply (order_preserving _). now apply precedes_flip.
   Qed.
 End order_preserving.
 
