src/implementations/nonneg_integers_naturals.v
@@ -64,7 +64,8 @@ Qed.
 Global Instance: NaturalsToSemiRing (Z⁺) := naturals.retract_is_nat_to_sr of_nat.
 Global Instance: Naturals (Z⁺) := naturals.retract_is_nat of_nat.
 
-Global Program Instance ZPos_cut_minus: CutMinus (Z⁺) := λ x y, if decide ('x ≤ 'y) then 0 else exist (λ z, 0 ≤ z) ('x - 'y) _.
+Global Program Instance ZPos_cut_minus `{∀ x y : Z, Decision (x ≤ y)} : CutMinus (Z⁺) 
+  := λ x y, if decide_rel (≤) ('x) ('y) then 0 else exist (λ z, 0 ≤ z) ('x - 'y) _.
 Next Obligation.
   apply <-rings.flip_nonneg_minus. 
   now apply orders.precedes_flip.
@@ -73,11 +74,11 @@ Qed.
 Global Instance: CutMinusSpec (Z⁺) ZPos_cut_minus.
 Proof.
   split; intros [x Ex] [y Ey] E1; unfold cut_minus, ZPos_cut_minus; unfold_equivs.
-   case (decide (x ≤ y)); intros E2.
+   case (decide_rel (≤) x y); intros E2.
     rewrite left_identity.
     now apply (antisymmetry o).
    simpl. ring.
-  case (decide (x ≤ y)); intros E2.
+  case (decide_rel (≤) x y); intros E2.
    reflexivity.
   simpl.
   apply (antisymmetry o).
